Книга вычислительная математика С. М. Устинов, В. А. зимницкий
5-6 расчетных заданий = зачёт 

1. $\displaystyle{\Delta\cos(k\alpha) = \cos((k+1)\alpha) - \cos(k\alpha) = \cos(k\alpha)\cos(\alpha) - \sin(k\alpha)\sin(\alpha) - \cos(k\alpha) = }$$\displaystyle{\cos(k\alpha)(\cos(\alpha)-1) - \sin(k\alpha)\sin(\alpha) = -2\cos(k\alpha)\left(\sin^2\left(\frac{\alpha}{2}\right)\right) - 2\sin(k\alpha)\sin(\frac{\alpha}{2})\cos(\frac{\alpha}{2})}$$\displaystyle{ = -2\sin(\frac{\alpha}{2})\left(\cos(k\alpha)\sin(\frac{\alpha}{2})+\cos(\frac{\alpha}{2})\sin(k\alpha) \right) = -2\sin(\frac{\alpha}{2})\left(\sin\left(k\alpha+\frac{\alpha}{2}\right) \right)}$


2. $\displaystyle{\Delta\cos\left(k\alpha - \frac{\alpha}{2} \right)}$
	 $\displaystyle{\Delta\cos\left(k\alpha - \frac{\alpha}{2} \right)= \cos\left((k+1)\alpha - \frac{\alpha}{2}\right) - \cos\left(k\alpha - \frac{\alpha}{2} \right) = \cos\left(k\alpha + \frac{\alpha}{2}\right) - \cos\left(k\alpha - \frac{\alpha}{2} \right) =}$$\displaystyle{\cos(k\alpha)\cos\left(\frac{\alpha}{2}\right) - \sin(k\alpha)\sin\left(\frac{\alpha}{2}\right) - \cos(k\alpha)\cos\left(\frac{\alpha}{2}\right) - \sin(k\alpha)\sin\left(\frac{\alpha}{2}\right) = -2\sin(k\alpha)\sin\left(\frac{\alpha}{2}\right)}$


3. $\displaystyle{\sum^n_{k=1}(2k-1)}$
	$\displaystyle{\sum^n_{k=1}(2k-1) = ((n+1)^2 - 2(n+1)) - (1-2) = n^2+2n+1-2n-2+1=n^2}$
	 $\displaystyle{\Delta f_k=k-1; \ f_k=Ck^2+Bk;\Delta f_k = C(k+1)^2+B(k+1) - Ck^2-Bk = Ck^2+2Ck+C+Bk+B-Ck^2-Bk = 2Ck + C + B}$
	${\begin{matrix} 2Ck + C + B = 2k-1 \\ \Bigg\{\begin{matrix} 2C = 2 \\ C+B = -1 \end{matrix}  \ \ \ \Bigg\{\begin{matrix} C = 1 \\ B = -2 \end{matrix} \Rightarrow f_k = k^2-2k \end{matrix}}$



4. $\displaystyle\sum^n_{k=1}(2k-1)^2$
	 $\displaystyle{\begin{matrix} \displaystyle\sum^n_{k=1}(2k-1)^2 = \frac{4}{3}(n+1)^3-4(n+1)^2+3\frac{2}{3}(n+1) - (\frac{4}{3} - 4 + 3\frac{2}{3}) = \\ \frac{4}{3}n^3 + 4n^2 + 4n + \frac{4}{3} - 4n^2 - 8n - 4 + 3\frac{2}{3}n + 3\frac{2}{3} - \frac{4}{3} + 4 - 3\frac{2}{3} =  \\ \frac{4}{3}n^3+\frac{1}{3}n = \frac{n(4n^2+1)}{3} \end{matrix}}$
	${\begin{matrix}\displaystyle\Delta f_k = 4k^2-4k+1; \ f_k =Dk^3+Ck^2+Bk \\ \Delta(Dk^3+Ck^2+Bk) = (D(k+1)^3+C(k+1)^2+B(k+1))-(D(k^3)+Ck^2+Bk) \\ =Dk^3+3Dk^2+3Dk+D+Ck^2+2Ck+C+Bk+B-Dk^3-Ck^2-Bk \\ =3Dk^2+3Dk+D+2Ck+C+B \\ \\ 3Dk^2+3Dk+D+2Ck+C+B = 4k^2-4k+1 \\ \Bigg\{\begin{matrix} 3D = 4 \\ 3D+2C = -4 \\ D+C+B = 1 \end{matrix} \ \ \ \Bigg\{\begin{matrix} D = \frac{4}{3} \\ C = -4 \\ B = 3\frac{2}{3} \end{matrix} \Rightarrow f_k = \frac{4}{3}k^2 - 4k + 3\frac{2}{3} \end{matrix}}$
5. Доказать: $\displaystyle{\sum^n_{k=1}k^3=\left(\sum^n_{k=1}k\right)^2=\frac{(n+1^2)n^2}{4}}$
	
